\input{../YKY-preamble.tex}

\title{Symmetric neural networks}
\author{YKY}

\begin{document}
\maketitle

\section{General case for $y = A x$}

\begin{equation}
\boxed{\mbox{original}} \quad y_j = \sum_i a_{ij} x_i .
\end{equation}

Equivariance implies:
\begin{eqnarray}
\boxed{\mbox{swapped}} \quad y_j ( \sigma(x_j \; x_k) x) &=& y_k \quad \boxed{\mbox{original}} \\
\sum_{i \neq j,k} a_{ij} x_i + a_{kj} x_j + a_{jj} x_k &=& \sum_{i \neq j,k} a_{ik} x_i + a_{jk} x_j + a_{kk} x_k . \nonumber
\end{eqnarray}

% for $(j \; k) \in \mathfrak{S}_n$.

Comparing coefficients yields:
\begin{eqnarray}
a_{ij} &=& a_{ik} \quad \quad \forall j, k, (i \neq j, k) \nonumber \\
a_{kj} &=& a_{jk} \quad \quad \forall j, k \nonumber \\
a_{jj} &=& a_{kk} \quad \quad \forall j, k .
\end{eqnarray}

In other words, the matrix $A$ is of the form:
\begin{equation}
A = \alpha I + \beta 1 1^T .
\end{equation}

\section{Case for $y_k = A_k x \cdot x$}

The general form of a ``quadratic'' vector function is:
\begin{equation}
y = (A x) \cdot x + B x + C .
\end{equation}

We just focus on the quadratic term $(A x) \cdot x$:
\begin{equation}
\boxed{\mbox{original}} \quad y_k = \sum_j \left[ \sum_i a_{ij}^k x_i \right] x_j .
\end{equation}

Equivariance implies:
\begin{eqnarray}
\boxed{\mbox{swapped}} \quad y_k ( \sigma(x_k \; x_h) x) &=& y_h \quad \boxed{\mbox{original}} \\
\sum_{j \neq h,k} \sum_{i \neq h,k} a_{ij}^k x_i x_j + a_{hh}^k x_k^2 + a_{kh}^k x_h x_k + a_{hk}^k x_k x_h + a_{kk}^k x_h^2 &=& \sum_{j \neq h,k} \sum_{i \neq h,k} a_{ij}^h x_i x_j + a_{hh}^h x_h^2 + a_{kh}^h x_k x_h + a_{hk}^h x_h x_k + a_{kk}^h x_k^2 \nonumber
\end{eqnarray}
which yields:
\begin{eqnarray}
a_{ij}^h &=& a_{ij}^k \quad \quad \forall h,k, (i,j) \neq (h,k) \nonumber \\
a_{hh}^h &=& a_{kk}^k \quad \quad \forall h,k \nonumber \\
a_{hh}^k &=& a_{kk}^h \quad \quad \forall h,k \nonumber \\
a_{kh}^k + a_{hk}^k &=& a_{kh}^h + a_{hk}^h \quad \quad \forall h,k .
\end{eqnarray}

\section{With output space ``folded in half''}

Now suppose the output is only $1/2$ the dimension of the input.  Define a new form of equivariance such that the input permutation would act on the output as ``folded in half''. 

In other words, equivariance is changed to:
\begin{equation}
\boxed{\mbox{swapped}} \quad y_k \cdot \sigma(x_k \; x_h) = y_h \mbox{  or  } y_{h-N/2} \quad \boxed{\mbox{original}} \end{equation}
where $\tau$ is $\sigma$ acting on $y$ as double its length and identifying $y_i = y_{i + N/2}$.

\subsection{Linear case}

Just notice that the dimension of $y$ is halved:
\begin{equation}
\boxed{\mbox{original}} \quad y_j = \sum_i a_{ij} x_i .
\end{equation}

``Folded'' equivariance implies:
\begin{eqnarray}
\boxed{\mbox{swapped}} \quad y_j ( \sigma(x_j \; x_k) x) \mbox{ or } y_m ( \sigma(x_m \; x_k) x) &=& y_k \mbox{ or } y_n \quad \boxed{\mbox{original}} \\
\sum_{i \neq j,k} a_{ij} x_i + a_{kj} x_j + a_{jj} x_k &=& \sum_{i \neq j,k} a_{ik} x_i + a_{jk} x_j + a_{kk} x_k  \nonumber \\
\mbox{or } \sum_{i \neq m,k} a_{im} x_i + a_{km} x_m + a_{mm} x_k & & \mbox{or } \sum_{i \neq j,n} a_{in} x_i + a_{jn} x_j + a_{nn} x_n  \nonumber
\end{eqnarray}
where $m = j - N/2, n = k - N/2$.  This gives rise to $2 \times 2 = 4$ cases.

Comparing coefficients yields:
\begin{eqnarray}
a_{ij} &=& a_{ik} \quad \quad \forall \;  j \le N/2, k \le N/2, (i \neq j, k) \nonumber \\
a_{kj} &=& a_{jk} \quad \quad \forall \;  j \le N/2, k \le N/2 \nonumber \\
a_{jj} &=& a_{kk} \quad \quad \forall \;  j \le N/2, k \le N/2 \nonumber\\
\hline \nonumber\\
a_{ij} &=& a_{ik} \quad \quad \forall \;  j > N/2, k \le N/2, (i \neq j, k) \nonumber \\
a_{kj} &=& a_{jk} \quad \quad \forall \;  j > N/2, k \le N/2 \nonumber \\
a_{jj} &=& a_{kk} \quad \quad \forall \;  j > N/2, k \le N/2 \nonumber\\
\hline \nonumber\\
a_{ij} &=& a_{ik} \quad \quad \forall \;  j \le N/2, k > N/2, (i \neq j, k) \nonumber \\
a_{kj} &=& a_{jk} \quad \quad \forall \;  j \le N/2, k > N/2 \nonumber \\
a_{jj} &=& a_{kk} \quad \quad \forall \;  j \le N/2, k > N/2 \nonumber\\
\hline \nonumber\\
a_{ij} &=& a_{ik} \quad \quad \forall \;  j > N/2, k > N/2, (i \neq j, k) \nonumber \\
a_{kj} &=& a_{jk} \quad \quad \forall \;  j > N/2, k > N/2 \nonumber \\
a_{jj} &=& a_{kk} \quad \quad \forall \;  j > N/2, k > N/2
\end{eqnarray}

\subsection{Quadratic case}

\end{document}